WIP

theories/PCUIC/QuoteGround.v
@@ -1,11 +1,13 @@
 From MetaCoq.Template Require Import utils All.
+From MetaCoq.PCUIC Require Import PCUICAst PCUICTyping Loader.
+From MetaCoq.PCUIC.PCUICTemplateMonad Require Import Core.
 Require Import Coq.Lists.List.
 Import ListNotations.
 
 Open Scope bs.
 Import MCMonadNotation.
 
-Class quotation_of {T} (t : T) := quoted_term_of : Ast.term.
+Class quotation_of {T} (t : T) := quoted_term_of : PCUICAst.term.
 Class ground_quotable T := quote_ground : forall t : T, quotation_of t.
 #[export] Existing Instance quote_ground.
 
@@ -21,27 +23,17 @@ Proof.
            | my_Some v => tmReturn v
            | my_None => tmFail "No typeclass instance"
            end) in
-     match qt return TemplateMonad Ast.term with
+     match qt return TemplateMonad PCUICAst.term with
      | tSort _
      | tConst _ _
      | tConstruct _ _ _
-     | tInt _
-     | tFloat _
+     | tPrim _
      | tInd _ _
        => tmReturn qt
-     | tCast t kind v
-       => tmInferQuotation t
-     | tApp f args
+     | tApp f x
        => qf <- tmInferQuotation f;;
-          qargs <- list_rect
-                     (fun _ => _)
-                     (tmReturn [])
-                     (fun arg args qargs
-                      => qarg <- tmInferQuotation arg;;
-                         qargs <- qargs;;
-                         tmReturn (qarg :: qargs))
-                     args;;
-          tmReturn (tApp qf qargs)
+          qx <- tmInferQuotation x;;
+          tmReturn (tApp qf qx)
      | tProj proj t => tmFail "Proj is not reduced"
      | tRel n => tmFail "Rel is not ground"
      | tVar id => tmFail "Var is not ground"
@@ -98,23 +90,67 @@ Ltac make_quotation_of_goal _ :=
 #[export] Instance quote_inductive : ground_quotable inductive := (ltac:(induction 1; exact _)).
 #[export] Instance quote_case_info : ground_quotable case_info := (ltac:(induction 1; exact _)).
 #[export] Instance quote_projection : ground_quotable projection := (ltac:(induction 1; exact _)).
-#[export] Instance quote_PrimInt63_int : ground_quotable PrimInt63.int := tInt.
-#[export] Instance quote_PrimFloat_float : ground_quotable PrimFloat.float := tFloat.
+#[export] Instance quote_PrimInt63_int : ground_quotable PrimInt63.int := fun x => tPrim (_; primIntModel x).
+#[export] Instance quote_PrimFloat_float : ground_quotable PrimFloat.float := fun x => tPrim (_; primFloatModel x).
+Module Import BasicAst.
+  #[export] Instance quote_context_decl {A} {qA : quotation_of A} {quoteA : ground_quotable A} : ground_quotable (BasicAst.context_decl A) := (ltac:(induction 1; exact _)).
+  #[export] Instance quote_typ_or_sort_ {A} {qA : quotation_of A} {quoteA : ground_quotable A} : ground_quotable (BasicAst.typ_or_sort_ A) := (ltac:(induction 1; exact _)).
+End BasicAst.
 #[export] Instance quote_predicate {A} {qA : quotation_of A} {quoteA : ground_quotable A} : ground_quotable (predicate A) := (ltac:(induction 1; exact _)).
 #[export] Instance quote_branch {A} {qA : quotation_of A} {quoteA : ground_quotable A} : ground_quotable (branch A) := (ltac:(induction 1; exact _)).
 #[export] Instance quote_def {A} {qA : quotation_of A} {quoteA : ground_quotable A} : ground_quotable (def A) := (ltac:(induction 1; exact _)).
 #[export] Instance quote_mfixpoint {A} {qA : quotation_of A} {quoteA : ground_quotable A} : ground_quotable (mfixpoint A) := _.
+Module Import Primitive.
+  #[export] Instance quote_prim_tag : ground_quotable Primitive.prim_tag := (ltac:(induction 1; exact _)).
+End Primitive.
+Module Import PCUICPrimitive.
+  #[export] Instance quote_prim_model {A} {qA : quotation_of A} {quoteA : ground_quotable A} {t} : ground_quotable (PCUICPrimitive.prim_model A t) := (ltac:(induction 1; exact _)).
+  #[export] Instance quote_context_decl {A} {qA : quotation_of A} {quoteA : ground_quotable A} : ground_quotable (BasicAst.context_decl A) := (ltac:(induction 1; exact _)).
+  #[export] Instance quote_prim_val {A} {qA : quotation_of A} {quoteA : ground_quotable A} : ground_quotable (PCUICPrimitive.prim_val A) := @quote_sigT _ (PCUICPrimitive.prim_model A) _ _ _ _.
+End PCUICPrimitive.
 #[export] Instance quote_term : ground_quotable term.
 Proof.
   hnf. fix quote_term 1; change (ground_quotable term) in quote_term; destruct 1.
   all: make_quotation_of_goal ().
 Defined.
 
-Module Import BasicAst.
-  #[export] Instance quote_context_decl {A} {qA : quotation_of A} {quoteA : ground_quotable A} : ground_quotable (BasicAst.context_decl A) := (ltac:(induction 1; exact _)).
-  #[export] Instance quote_typ_or_sort_ {A} {qA : quotation_of A} {quoteA : ground_quotable A} : ground_quotable (BasicAst.typ_or_sort_ A) := (ltac:(induction 1; exact _)).
-End BasicAst.
+Module Export PCUICEnvironment.
+  #[export] Instance quote_context : ground_quotable PCUICAst.PCUICEnvironment.context := _.
+End PCUICEnvironment.
 
-Module Import Primitive.
-  #[export] Instance quote_prim_tag : ground_quotable Primitive.prim_tag := (ltac:(induction 1; exact _)).
-End Primitive.
+Module Import PCUICTyping.
+  #[export] Instance quote_All_local_env {typing} {qtyping : quotation_of typing} {quote_typing : forall Γ t T, ground_quotable (typing Γ t T)} {Γ} {qΓ : quotation_of Γ} : ground_quotable (@PCUICTyping.All_local_env typing Γ) := (ltac:(induction 1; exact _)).
+  #[local] Hint Extern 1 (_ = _) => reflexivity : typeclass_instances.
+  #[export] Instance quote_lift_judgment {check infer_sort}
+   {Σ Γ t T}
+   {quote_check : forall T', Typ T' = T -> ground_quotable (check Σ Γ t T')}
+   {quote_infer_sort : T = Sort -> ground_quotable (infer_sort Σ Γ t)}
+    : ground_quotable (@PCUICTyping.lift_judgment check infer_sort Σ Γ t T)
+    := (ltac:(cbv [PCUICTyping.lift_judgment]; exact _)).
+  #[export] Instance quote_infer_sort {sorting} {Σ Γ T} {qsorting : quotation_of (sorting Σ Γ T)} {quote_sorting : forall U, quotation_of U -> ground_quotable (sorting Σ Γ T U)} : ground_quotable (@PCUICTyping.infer_sort sorting Σ Γ T) := @quote_sigT _ (sorting Σ Γ T) _ _ _ _.
+  #[local] Instance quotation_of_compose_tSort {A} (f : _ -> A) {qf : quotation_of f} : quotation_of (fun s => f (tSort s)).
+  Proof.
+    lazymatch constr:(<% fun s => f (tSort s) %>) with
+    | context qt[tVar "f"]
+      => let qt := context qt[qf] in
+         exact qt
+    end.
+  Defined.
+  #[local] Hint Extern 1 => progress (intros; subst) : typeclass_instances.
+  #[export] Instance quote_lift_typing {typing} {Σ Γ t T}
+   {quote_typing : forall T', Typ T' = T -> ground_quotable (typing Σ Γ t T')}
+   {quote_typing' : forall U, T = Sort -> quotation_of U -> ground_quotable (typing Σ Γ t (tSort U))}
+   {qtyping : T = Sort -> quotation_of (typing Σ Γ t)}
+    : ground_quotable (@PCUICTyping.lift_typing typing Σ Γ t T)
+    := ltac:(cbv [PCUICTyping.lift_typing]; exact _).
+  #[export] Instance quote_typing {checker_flags Σ Γ x T} : ground_quotable (@PCUICTyping.typing checker_flags Σ Γ x T).
+  Proof.
+    hnf. fix quote_typing 1; change (ground_quotable (@PCUICTyping.typing checker_flags Σ Γ x T)) in quote_typing; destruct 1.
+    Typeclasses eauto := debug.
+    all: try make_quotation_of_goal ().
+    pose (_ : quotation_of n).
+    pose (_ : quotation_of decl).
+    pose (_ : quotation_of e).
+    pose (_ : quotation_of a).
+  Defined.
+Inductive typing `{checker_flags} (Σ : global_env_ext) (Γ : context) : term -> term -> Type :=
